\section{Conditional Probability}

\subsection{Conditional Probability}

\subsubsection*{Conditional Probability}
\begin{itemize}
    \item \textbf{Def.} For events $A$, $B$ with $P(B)>0$, probability of $A$ given $B$, $P(A\mid B)$ is
    \begin{equation}\label{eq:prp:cond-prob}
        P(A\mid B):=\frac{P(A\cap B)}{P(B)}~~(P(B)>0)
    \end{equation}
    \item $P(A)$: prior probability
    \item $P(B)$: evidence probability
    \item $P(A\mid B)$: posterior probability
\end{itemize}

\subsubsection*{Bayes' Rule}
\begin{itemize}
    \item $P(A_1,A_2,\cdots,A_n)=P(A_1\cap A_2\cap\cdots A_n)$
    \item For any events $A$, $B$ with $P(A)>0$ and $P(B)>0$,
    \begin{equation}\label{eq:prp:cond-prob-both-sides}
        P(A\cap B)=P(B)P(A\mid B)=P(A)P(B\mid A)
    \end{equation}
    \begin{itemize}
        \item Derived from \ref{eq:prp:cond-prob}
    \end{itemize}
    \item For any events with $A_1,A_2,\cdots,A_n$ s.t. $P(A_i)>0$,
    \begin{equation}
        P(A_1,A_2,\cdots,A_n)=P(A_1)P(A_2\mid A_1)P(A_3\mid A_1,A_2)\cdots P(A_n\mid A_1,\cdots,A_{n-1})
    \end{equation}
    \item Bayes' Rule: Derived from \ref{eq:prp:cond-prob-both-sides}
    \begin{equation}\label{eq:prp:bayes-rule}
        P(A\mid B)=\frac{P(B\mid A)P(A)}{P(B)}
    \end{equation}
\end{itemize}

\subsubsection*{Law of total probability (LOTP)}
\begin{itemize}
    \item Let $A_1,A_2,\cdots,A_n$ be a partition of the sample space $S$, i.e. $S=\dot{\bigcup}_{i=1}^nA_i$, then
    \begin{equation}
        P(B)=\sum_{i=1}^nP(B\mid A_i)P(A_i)
    \end{equation}
    \item For an event $A\subset S$,
    \begin{equation}
        P(B)=P(B\mid A)P(A)+P(B\mid A^c)P(A^c)
    \end{equation}
\end{itemize}

\subsubsection*{Conditional Probability and Likelihood Function}
\begin{itemize}
    \item For a given event $E\subset S$ with $P(E)>0$,
    \item $P(\cdot\mid E)$ is a probability function
    \begin{itemize}
        \item $\because$ $P(S\mid E)=1$ and satisfies LOTP.
        \item $P(A^c\mid E)=1-P(A\mid E)$, $P(\emptyset\mid E)=0$, $P(A\cup B\mid E)=P(A\mid E)+P(B\mid E)-P(A\cap B\mid E)$
    \end{itemize}
    \item $P(E\mid\cdot)$ is NOT a probability function; Instead, a ``likelihood function''
    \begin{itemize}
        \item $P(E\mid\emptyset)$ cannot be defined, $P(E\mid S)=P(E)\neq 1$
    \end{itemize}
\end{itemize}

\subsubsection*{Extra Conditioning}
\begin{itemize}
    \item Bayes' rule w/ extra conditioning: $P(A\cap E)>0$ and $P(B\cap E)>0$, then
    \begin{equation}
        P(A\mid B,E)=\frac{P(B\mid A,E)P(A\mid E)}{P(B\mid E)}
    \end{equation}
    \begin{itemize}
        \item \ref{eq:prp:bayes-rule} is when $E=S$
    \end{itemize}
    \item LOTP w/ extra conditioning: For $A_i$ s.t. $S=\dot{\bigcup}_{i=1}^nA_i$ and $P(A_i\cap E)>0$,
    \begin{equation}
        P(B\mid E)=\sum_{i=1}^nP(B\mid A_i,E)P(A_i,E)
    \end{equation}
\end{itemize}

\subsubsection*{Independence}
\begin{itemize}
    \item \textbf{Def.} Events $A$ and $B$ are independent if
    \begin{equation}
        P(A\cap B)=P(A)P(B)
    \end{equation}
    \begin{itemize}
        \item Notation: $A\indep B$
        \item $A\indep B$ $\implies$ $P(A\mid B)=P(A)$, $P(B\mid A)=P(B)$
        \item Mutually exclusive events ($A\cap B=\emptyset$) DOES NOT imply independence
        \item Mutually exclusive: $P(A\mid B)=0$, Equal: $P(A\mid B)=1$, Independent: $P(A\mid B)=P(A)$
    \end{itemize}
    \item $A\indep B$ $\implies$ $A^c\indep B$, $A\indep B^c$, $A^c\indep B^c$
    \item \textbf{Def.} Independence of many events: $n$ events $A_1,A_2,\cdots,A_n$ are independent if
    \begin{equation}
        \forall~\{i_1,\cdots,i_k\}\subset\{1,\cdots,n\},~P\left(\bigcap_{j=1}^kA_{i_j}\right)=\prod_{j=1}^kP(A_{i_j})
    \end{equation}
    \item \textbf{Def.} Conditional indep.: Events $A$, $B$: cond. indep. given $E$ if
    \begin{equation}
        P(A\cap B\mid E)=P(A\mid E)P(B\mid E)
    \end{equation}
    \begin{itemize}
        \item Notation: $A\indep B\mid E$
        \item Pairwise independence (e.g. $A$-$B$, $B$-$C$, $C$-$A$) $\centernot\implies$ Independence
        \item Conditional Independence $\centernot\iff$ Independence
    \end{itemize}
\end{itemize}
