\section{Joint Distributions}

\subsection{Joint Distributions}

\subsubsection*{Joint, Marginal, Conditional PMF}
\begin{itemize}
    \item Joint CDF of r.v.s $X$ and $Y$
    \begin{equation}
        F_{X,Y}(x,y)=P(X\leq x,Y\leq y)
    \end{equation}
    \item Joint PMF of discrete r.v.s $X$ and $Y$
    \begin{equation}
        p_{X,Y}(x,y)=P(X=x,Y=y)
    \end{equation}
    \item Marginal PMF of $X$ for discrete r.v.s $X$ and $Y$
    \begin{equation}
        P(X=x)=\sum_yP(X=x,Y=y)
    \end{equation}
    \item Conditional PMF of discrete r.v.s $Y$ given $X=x$
    \begin{equation}
        P_{Y\mid X=x}(y)=P(Y=y\mid X=x)=\frac{P(X=x,Y=y)}{P(X=x)}
    \end{equation}
\end{itemize}

\subsubsection*{Joint, Marginal, Conditional PDF}
\begin{itemize}
    \item Joint PDF of continuous r.v. $X$, $Y$ is a derivative of its CDF
    \begin{equation}
        f_{X,Y}(x,y)=\frac{\partial^2}{\partial x\partial y}F_{X,Y}(x,y)
    \end{equation}
    \item Valid PDF: $f_{X,Y}(x,y)\geq 0$ and $\iint_{\mathbb{R}^2}f_{X,Y}(x,y)~dA=1$
    \item For a general set $A\subset\mathbb{R}^2$,
    \begin{equation}
        P((X,Y)\in A)=\iint_Af_{X,Y}(x,y)~dA
    \end{equation}
    \item Marginal PDF of $X$ for continuous r.v.s $X$ and $Y$
    \begin{equation}
        f_X(x)=\int_{-\infty}^{\infty}f_{X,Y}(x,y)~dy
    \end{equation}
    \item Conditional PDF of continuous r.v.s $Y$ given $X=x$
    \begin{equation}
        f_{Y\mid X}(y\mid x)=\frac{f_{X,Y}(x,y)}{f_X(x)}
    \end{equation}
\end{itemize}
\clearpage

\subsubsection*{Generalization of Probability Rules}
\begin{itemize}
    \item Bayes' Rule
    \begin{equation}
        f_{Y\mid X}(y\mid x)=\frac{f_{X\mid Y}(x\mid y)f_Y(y)}{f_X(x)}
    \end{equation}
    \item LOTP
    \begin{equation}
        f_X(x)=\int_{-\infty}^{\infty}f_{X\mid Y}(x\mid y)f_Y(y)~dy
    \end{equation}
    \item 2D LOTUS
    \begin{equation}
        E(g(X,Y))=\int_{-\infty}^\infty\int_{-\infty}^\infty g(x,y)f_{X,Y}(x,y)~dxdy
    \end{equation}
    \begin{itemize}
        \item Discrete version: $E(g(X,Y))=\sum_x\sum_yg(x,y)P(X=x,Y=y)$
    \end{itemize}
\end{itemize}

\subsubsection*{Independence of Random Variables}
\begin{itemize}
    \item Random variables $X$ and $Y$ are independent if
    \begin{equation}\label{eq:prp:rv-indep}
        \forall~x,y,~F_{X,Y}(x,y)=F_X(x)F_Y(y)
    \end{equation}
    \item $X$, $Y$: discrete
    \begin{itemize}
        \item \ref{eq:prp:rv-indep} $\iff$ $p_{X,Y}(x,y)=p_X(x)p_Y(y)$
        \item \ref{eq:prp:rv-indep}, $P(X=x)>0$ $\iff$ $P(Y=y\mid X=x)=P(Y=y)$
    \end{itemize}
    \item $X$, $Y$: continuous
    \begin{itemize}
        \item \ref{eq:prp:rv-indep} $\iff$ $f_{X,Y}(x,y)=f_X(x)f_Y(y)$
        \item \ref{eq:prp:rv-indep}, $f_X(x)>0$ $\iff$ $f_{Y\mid X}(y\mid x)=f_Y(y)$
        \item Joint PDF $f_{X,Y}$ can be factorized into two nonnegative functions $\iff$ $X\indep Y$
    \end{itemize}
\end{itemize}

\subsubsection*{Covariance}
\begin{itemize}
    \item Covariance between r.v.s $X$ and $Y$
    \begin{equation}
        \text{Cov}(X,Y):=E\Bigr[(X-E(X))(Y-E(Y))\Bigr]=E(XY)-E(X)E(Y)
    \end{equation}
    \item $X\indep Y\implies\text{Cov}(X,Y)=0$
    \begin{itemize}
        \item $\text{Cov}(X,Y)=0$ $\implies$ $X$ and $Y$ are \textit{uncorrelated}
        \item Converse is false
    \end{itemize}
    \item Properties: For any r.v.s $X$, $Y$, $Z$, $W$ and constant $c\in\mathbb{R}$,
    \begin{itemize}
        \item $\text{Cov}(X,X)=\text{Var}(X)$
        \item $\text{Cov}(X,Y)=\text{Cov}(Y,X)$
        \item $\text{Cov}(X,c)=0$
        \item $\text{Cov}(cX,Y)=c\text{Cov}(X,Y)$
        \item $\text{Cov}(X+Y,Z)=\text{Cov}(X,Z)+\text{Cov}(Y,Z)$
        \item $\text{Cov}(X+Y,Z+W)=\text{Cov}(X,Z)+\text{Cov}(X,W)+\text{Cov}(Y,Z)+\text{Cov}(Y,W)$
        \item $\text{Var}(X\pm Y)=\text{Var}(X)+\text{Var}(Y)\pm 2\text{Cov}(X,Y)$
        \item $\text{Var}\left(\sum_{i=1}^nX_i\right)=\sum_{i=1}^n\text{Var}(X_i)+2\sum_{i<j}\text{Cov}(X_i,X_j)$
    \end{itemize}
    \item Correlation between r.v.s $X$ and $Y$
    \begin{equation}
        \text{Corr}(X,Y):=\frac{\text{Cov}(X,Y)}{\sqrt{\text{Var}(X)\text{Var}(Y)}}
    \end{equation}
    \begin{itemize}
        \item Undefined if $\text{Var}(X)=0$ or $\text{Var}(Y)=0$
        \item \textit{Normalized} covariance: $\forall~X,Y$, $\abs{~\text{Corr}(X,Y)~}\leq 1$
    \end{itemize}
\end{itemize}

\subsubsection*{Joint MGF}
\begin{itemize}
    \item Joint MGF of random vector $\mathbf{X}=\left(X_1,X_2,\cdots,X_k\right)$ of $\mathbf{t}=\left(t_1,t_2,\cdots,t_k\right)$ is
    \begin{equation}
        M_{\mathbf{X}}(\mathbf{t})=E\left(e^{\mathbf{t}^T\mathbf{X}}\right)=E\left(e^{\sum_{i=1}^kt_iX_i}\right)
    \end{equation}
    \begin{itemize}
        \item MGF for joint distribution
        \item $\mathbf{X}$: independent r.v.s $\iff$ Joint MGF: given as product of MGFs
        \begin{equation}
            M_{\mathbf{X}}(\mathbf{t})=E\left(\prod_{i=1}^ke^{t_iX_i}\right)=\prod_{i=1}^kM_{X_i}(t_i)
        \end{equation}
    \end{itemize}
\end{itemize}

\subsubsection*{Multivariate Normal (MVN, Jointly Gaussian)}
\begin{itemize}
    \item Random vector $\mathbf{X}=\left(X_1,X_2,\cdots,X_k\right)$: MVN distribution if
    \begin{equation}
        \forall~t_1,t_2,\cdots,t_k\in\mathbb{R},~\sum_{i=1}^kt_iX_i\sim\mathcal{N}
    \end{equation}
    \begin{itemize}
        \item $k=2$: $\mathbf{X}$ has Bivariate Normal (BVN)
        \item $\mathbf{X}$: MVN $\implies$ $\forall X_i$: Normal
        \item $\forall X_i$: Normal $\centernot\implies$ $\mathbf{X}$: MVN
        \item Within MVN $\mathbf{X}$, $\text{Cov}(X_i,X_j)=0$ $\implies$ $X_i\indep X_j$
    \end{itemize}
    \item MVN $\mathbf{X}$ is denoted by
    \begin{equation}
        \mathbf{X}\sim\mathcal{N}(\mu,\Sigma_\mathbf{X})
    \end{equation}
    \begin{itemize}
        \item Mean vector $\mu=\left(\mu_1,\mu_2,\cdots,\mu_k\right)$
        \item Covariance matrix: outer product of $\mathbf{X}-\mu$
        \begin{equation}
            \Sigma_\mathbf{X}=E\left((\mathbf{X}-\mu)(\mathbf{X}-\mu)^T\right)=\begin{mtx}{cccc}
                \text{Var}(X_1) & \text{Cov}(X_1,X_2) & \cdots & \text{Cov}(X_1,X_n) \\
                \text{Cov}(X_2,X_1) & \text{Var}(X_2) & \cdots & \text{Cov}(X_2,X_n) \\
                \vdots & \vdots & \ddots & \vdots \\
                \text{Cov}(X_n,X_1) & \text{Cov}(X_n,X_2) & \cdots & \text{Var}(X_n)
            \end{mtx}
        \end{equation}
    \end{itemize}
    \item PDF of MVN $\mathbf{X}$
    \begin{equation}
        f_{\mathbf{X}}(\mathbf{x})=\frac{1}{\sqrt{(2\pi)^n\abs{\text{det}\Sigma_\mathbf{X}}}}\exp\left(-\frac{1}{2}(\mathbf{x-\mu})^T\Sigma_\mathbf{X}^{-1}(\mathbf{x-\mu})\right)
    \end{equation}
\end{itemize}
